\documentclass[Lecture.tex]{subfiles}
\begin{document}
\section{3.1: Derivatives of Polynomials}
\subsection{Constants}
\begin{frame}{Derivative of Constants}
  \begin{itemize}
  \item<1->
    Let $f(x) = a$ for $a \in \R$ (this means ``a is an element of $\R$'', the set of real numbers).
  \item<2->
    The difference quotient for any $x_0, x_1$ is
    $$\onslide<2->{\frac{f(x_0) - f(x_1)}{x_0 - x_1}}\onslide<3->{= \frac{a - a }{x_0 - x_1}}\onslide<4->{ = 0.}$$
  \item<5->
    Therefore $f^\prime(x) = 0$.
  \end{itemize}
\end{frame}

\subsection{Linearity}
\begin{frame}{The Derivative is a Linear Operator}
  Let $f$ and $g$ be differentiable functions, and let $a \in \R$.
  \begin{itemize}
  \item<2->
    $$\ddx{x}\left(f(x) \pm g(x)\right) \onslide<3->{= \ddx{x}f(x) \pm \ddx{x}g(x)}$$
  \item<4->
    $$\frac{\operatorname{d}}{\operatorname{dx}}\left(af(x)\right) \onslide<5->{= a \ddx{x}f(x).}$$
  \end{itemize}
\end{frame}

\subsection{Power Rule}

\begin{frame}{Derivative of a Power Functions}
  The derivative of $x^n$ for $n \in \R$ is 
  $$\ddx{x}\left(x^n\right) = nx^{n-1}.$$

  \onslide<2->{
    \begin{rmk}
      The derivative of a linear function is
      $$\ddx{x}\left(mx + b\right) = m\ddx{x}x + \ddx{x}(b) = m$$
    \end{rmk}
  }
\end{frame}

\begin{frame}{Derivative of Polynomials}
  Consider a degree $n$ polynomial,
  $$p(x) = a_nx^n + a_{n-1}x^{n-1} + \cdots + a_2x^2 + a_1x + a_0.$$
  \onslide<2->{The derivative is
    \begin{eqnarray*}
      p^\prime(x) &=& \ddx{x}(a_nx^n + a_{n-1}x^{n-1} + \cdots + a_2x^2 + a_1x + a_0) \\
      \onslide<2->{&=& a_n\ddx{x}(x^n) + a_{n-1}\ddx{x}(x^{n-1}) + \cdots\\
        &+& a_2\ddx{x}(x^2) + a_1\ddx{x}(x)\\}
      \onslide<3->{&=& na_nx^{n-1} + (n-1)a_{n-1}x^{n-2} + \cdots + 2a_2x + a_1.}
    \end{eqnarray*}
  }
\end{frame}

\begin{frame}{Example}
  Differentiate the following
  \begin{multicols}{2}
    \begin{enumerate}
    \item<alert@2-6>
      $A(t) = 3t^5$
    \item<alert@7-10>
      $r(p) = p^5 + p^3$
    \item<alert@11-16>
      $f(x) = 5x^2 - 7x^3$
    \item<alert@17->
      $g(t) = \frac{t^2}{4} + 3$
    \end{enumerate}
  \end{multicols}
  
  \begin{minipage}[t]{\linewidth}
    \only<2-6>{
      \begin{eqnarray*}
        A^\prime(t) &=& \onslide<3->{\ddx{t}\left(3t^5\right)}\\
        \onslide<4->{&=& 3 \left(\ddx{t}\left(t^5\right)\right)\\}
        \onslide<5->{&=& 3 \left(5 t^4\right)\\}
        \onslide<6->{&=& 15 t^4.}
      \end{eqnarray*}
    }
    \only<7-10>{
      \begin{eqnarray*}
        \onslide<7->{r^\prime(p) &=&}
        \onslide<8->{\ddx{p}\left(p^5 + p^3\right)\\}
        \onslide<9->{&=& \ddx{p}\left(p^5\right) + \ddx{p}\left(p^3\right)\\}
        \onslide<10->{&=& 5p^4 + 3p^2.}
      \end{eqnarray*}
    }
    \only<11-16>{
      \begin{eqnarray*}
        \onslide<11->{f^\prime(x) &=& }
        \onslide<12->{\ddx{x}\left(5x^2 - 7x^3\right)}
        \onslide<13->{=\ddx{x}\left(5x^2\right) - \ddx{x}\left(7x^3\right)\\}
        \onslide<14->{&=& 5\ddx{x}\left(x^2\right) - 7\ddx{x}\left(x^3\right)}
        \onslide<15->{= 5(2x) - 7(3x^2)\\}
        \onslide<16->{&=& 10x - 21x^2.}
      \end{eqnarray*}
    }
    \only<17->{
      \begin{eqnarray*}
        \onslide<17->{g^\prime(t) &=&}
        \onslide<18->{\ddx{t}\left(\frac{t^2}{4} + 3\right)}
        \onslide<19->{= \ddx{t}\left(\frac{t^2}{4}\right) + \ddx{t}\left(3\right)\\}
        \onslide<20->{&=& \frac{1}{4}\ddx{t}\left(t^2\right) + 0\\}
        \onslide<21->{&=& \frac{1}{4}\left(2t\right)\\}
        \onslide<22->{&=& \frac{t}{2}.}
      \end{eqnarray*}
    }
  \end{minipage}

\end{frame}

\begin{frame}{Example}
  Find the derivative of
  $$f(x) = x^3 - 2x^2 - 5x + 7.$$
  
  \begin{eqnarray*}
    \onslide<2->{f^\prime(x) &=& \ddx{x}(x^3 - 2x^2 - 5x + 7)\\}
    \onslide<3->{&=& \ddx{x}(x^3) - \ddx{x}(2x^2) - \ddx{x}(5x) + \ddx{x}(7)\\}
    \onslide<4->{&=& \ddx{x}(x^3) - 2\ddx{x}(x^2) - 5\ddx{x}(x) + 0\\}
    \onslide<5->{&=& 3x^2 - 4x - 5.}
  \end{eqnarray*}
\end{frame}
\end{document}
